examples/steel/Selectors.LList.Derived.fst
@@ -1,0 +1,26 @@
+module Selectors.LList.Derived
+
+let push p x =
+  let c = mk_cell p x in
+  let head = alloc c in
+  intro_llist_cons head p;
+  head
+
+let pop #a p =
+  let h0 = get #(llist p) () in
+  let tl = tail p in
+  let x = read p in
+  let v = data x in
+  free p;
+  let h1 = get #(llist tl) () in
+  let l = Ghost.hide (v_llist tl h1) in
+  change_slprop (llist tl) (llist (Res?.n (Res v tl))) l l (fun _ -> ());
+  Res v tl
+
+let rec length #a p =
+  if is_null p then (elim_llist_nil p; 0)
+  else (
+    let tl = tail p in
+    let aux = length tl in
+    intro_llist_cons p tl;
+    1 + aux)
