examples/steel/Selectors.LList.Derived.fsti
@@ -1,0 +1,33 @@
+module Selectors.LList.Derived
+
+open Steel.SelEffect
+
+open Selectors.LList
+module L = FStar.List.Tot
+
+val push (#a:Type0) (p:t a) (x: a)
+  : SteelSel (t a) (llist p) (fun n -> llist n)
+             (requires fun _ -> True)
+             (ensures fun h0 n h1 -> v_llist n h1 == x::v_llist p h0)
+
+//AF: Using a pair instead leads to a CheckUVar error in the implementation
+// Additional problem: The projectors are not reduced, it seems the attribute it not propagated
+[@@__steel_reduce__]
+noeq
+type res (a:Type0) = | Res: x:a -> n:t a -> res a
+
+val pop (#a:Type0) (p:t a)
+  : SteelSel (res a) (llist p) (fun res -> llist (res.n))
+             (requires fun _ -> p =!= null_llist)
+             (ensures fun h0 res h1 -> (
+               let l = v_llist p h0 in
+               Cons? l /\
+               res.x == L.hd l /\
+               v_llist res.n h1 == L.tl l))
+
+val length (#a:Type0) (p:t a)
+  : SteelSel int (llist p) (fun _ -> llist p)
+             (requires fun _ -> True)
+             (ensures fun h0 x h1 ->
+               v_llist p h0 == v_llist p h1 /\
+               L.length (v_llist p h0) == x)
